Add polished (more-or-less) lemmas for sharpening stateful filters

src/packet_filters.v
@@ -6,7 +6,8 @@ Require Import Coq.Lists.List.
 Import ListNotations.
 Require Import Fiat.QueryStructure.Automation.MasterPlan.
 Require Import IndexedEnsembles.
-Require Import Fiat.Narcissus.Examples.IPTables.
+Require Import Fiat.Narcissus.Examples.Guard.IPTables.
+Require Import Fiat.Narcissus.Examples.Guard.PacketFiltersLemmas.
 
 Definition sINPUT := "Input".
 Definition sHISTORY := "GlobalHistory".
@@ -79,6 +80,7 @@ Proof.
     | rewrite <- GetRelDropConstraints; apply Hbin | apply Hbres].
 Qed.
 
+
 Definition NoIncomingConnectionsFilter : ADT StatefulFilterSig :=
   Eval simpl in Def ADT {
     rep := QueryStructure PacketHistorySchema,
@@ -95,146 +97,6 @@ Lemma simpl_in_bind:
     In T (`(r', _) <- ret (x, y); ret r') v -> x = v.
 Proof.
   intros. apply Bind_inv in H. destruct H. destruct H. apply Return_inv in H. rewrite <- H in H0. simpl in H0. apply Return_inv in H0. assumption. Qed.
-
-Definition UnIndexedEnsembleListEquivalence'
-           (ElementType : Type)
-           (ensemble : IndexedEnsemble)
-           (l : list ElementType) :=
-  sig (fun (l': list IndexedElement) =>
-         map indexedElement l' = l /\
-         (forall x : IndexedElement,
-            In IndexedElement ensemble x <-> List.In x l') /\
-         NoDup (map elementIndex l')).
-
-
-Definition AllFinite {qs_schema} (r: UnConstrQueryStructure qs_schema) :=
-  forall idx, {l: list RawTuple & UnIndexedEnsembleListEquivalence' _ (GetUnConstrRelation r idx) l}.
-
-Definition FiniteTables_AbsR'
-    {qs_schema}
-    (r_o : UnConstrQueryStructure qs_schema)
-    (r_n : { r_n: UnConstrQueryStructure qs_schema & AllFinite r_n }) :=
-  r_o = projT1 r_n.
-
-Lemma QSEmptyIsFinite {qs_schema}: AllFinite (DropQSConstraints (QSEmptySpec qs_schema)).
-Proof.
-  unfold AllFinite. intros. exists []. exists [].
-  split. reflexivity. split. split; intros.
-(*  pose proof (FiniteEnsemble_QSEmptySpec idx) as Hfin. red in Hfin.
-  destruct Hfin as [l Hl]. red in Hl. destruct Hl as [l' [Hmap [Heqv Hdup]]]. *)
-  unfold In, GetUnConstrRelation, DropQSConstraints, QSEmptySpec in H. simpl in H.
-
-
-  Coercion mycoer {qs_schema idx t}
-           (y: @IndexedElement
-                 (@RawTuple
-                    (@GetNRelSchemaHeading
-                       (numRawQSschemaSchemas
-                          (QueryStructureSchemaRaw qs_schema))
-                       (qschemaSchemas (QueryStructureSchemaRaw qs_schema)) idx))) :
-    @IndexedRawTuple
-      (rawSchemaHeading
-         (@Vector.nth RawSchema (numQSschemaSchemas qs_schema) t idx)).
-  Admitted.
-
-  assert (Hscraw: qschemaSchemas qs_schema = Vector.map schemaRaw (QSschemaSchemas qs_schema)).
-  { reflexivity. }
-
-  replace x with (@mycoer _ _ (@Vector.map Schema RawSchema schemaRaw (numQSschemaSchemas _) (QSschemaSchemas _)) x) in H.
-  rewrite <- Hscraw in H. rewrite <- ith_imap2 in H.
-  Set Printing All. Check (Build_EmptyRelation_IsEmpty qs_schema idx). simpl in H. admit. admit.
-  (*replace (fun ns: RawSchema => RawRelation ns) with RawRelation in H. rewrite Build_EmptyRelation_IsEmpty in H.*)
-  inversion H. constructor.
-Qed.
-Unset Printing All.
-
-Lemma FiniteTables_AbsR'_QSEmptySpec
-      {qs_schema}
-  :  FiniteTables_AbsR'
-       (DropQSConstraints (QSEmptySpec qs_schema))
-       (existT AllFinite (DropQSConstraints (QSEmptySpec qs_schema)) QSEmptyIsFinite).
-Proof. reflexivity. Qed.
-
-Lemma change_refine_form {X1 X2 Y Z} :
-  forall (cx: Comp (X1 * X2)) (cy: X1 * X2 -> Comp Y) (f: Y -> Comp Z),
-    refine
-      (x <- cx;
-       y <- cy x;
-       f y)
-      (x0 <- (x <- cx;
-              y <- cy x;
-              ret (y, snd x));
-       f (fst x0)).
-Proof.
-  intros.
-  unfold refine; intros.
-  computes_to_inv; subst.
-  eauto.
-Qed.
-
-
-Lemma insert_finite_helper:
-  forall (qs_schema : RawQueryStructureSchema)
-         (r_n: { r_n: UnConstrQueryStructure qs_schema & AllFinite r_n })
-         idx tup,
-    UnConstrFreshIdx (GetUnConstrRelation (projT1 r_n) idx) (elementIndex tup) ->
-    AllFinite (UpdateUnConstrRelation (projT1 r_n) idx
-                 (EnsembleInsert tup (GetUnConstrRelation (projT1 r_n) idx))).
-Proof.
-  red; intros qsc r_n idx tup Hfresh idx'. destruct (Fin.eqb idx idx') eqn:idxeq.
-  - apply Fin.eqb_eq in idxeq. subst idx'.
-    destruct r_n as [r Hfin]. destruct (Hfin idx) as [l1 Hl1].
-    destruct Hl1 as [l2 [Hmap [Hin Hdup]]].
-    exists ((indexedElement tup) :: l1). cbn.
-    rewrite get_update_unconstr_eq. red. exists (tup :: l2).
-    
-    split. simpl. rewrite <- Hmap. reflexivity. split.
-    split; intros H; unfold EnsembleInsert, In in *;
-      destruct H; simpl;
-        [ left; symmetry; assumption
-        | right; apply (Hin x); apply H
-        | left; symmetry; assumption
-        | right; apply (Hin x); apply H].
-    
-    simpl. apply NoDup_cons. red in Hfresh. simpl in Hfresh.
-    assert (Hlist: forall (x: nat) l,
-               (forall x', List.In x' l -> lt x' x) ->
-               ~List.In x l).
-    {
-      intros x l Hx'. intro Hx. apply (Hx' x) in Hx.
-      apply lt_irrefl in Hx. inversion Hx.
-    }
-    apply Hlist. apply forall_In_map. intros elem Helem.
-    apply Hfresh. apply (Hin elem).
-    assumption. assumption.
-    
-  - assert (Hidxeq: idx <> idx').
-    { intro. apply Fin.eqb_eq in H. congruence. }
-    destruct r_n as [r Hfin]. destruct (Hfin idx') as [l1 Hl1].
-    exists l1. cbn. rewrite get_update_unconstr_neq.
-    assumption. assumption.
-Qed.
-
-Lemma FiniteTables_AbsR'_Insert :
-  forall (qs_schema : RawQueryStructureSchema) r_o r_n
-         (idx : Fin.t (numRawQSschemaSchemas qs_schema)) tup,
-    FiniteTables_AbsR' r_o r_n ->
-    UnConstrFreshIdx (ith2 r_o idx) (elementIndex tup) ->
-    forall (H: UnConstrFreshIdx (GetUnConstrRelation (projT1 r_n) idx) (elementIndex tup)),
-    refine
-      {r_n0 : { r_n: UnConstrQueryStructure qs_schema & AllFinite r_n } |
-       FiniteTables_AbsR'
-         (UpdateUnConstrRelation r_o idx (EnsembleInsert tup (GetUnConstrRelation r_o idx))) r_n0}
-      (ret (existT AllFinite
-              (UpdateUnConstrRelation (projT1 r_n) idx
-                 (EnsembleInsert tup (GetUnConstrRelation (projT1 r_n) idx)))
-              (insert_finite_helper _ _ _ _ H))).
-Proof.
-  intros qsc r_o r_n idx tup Hrel Hfresho Hfreshn.
-  unfold refine; intros r_n' Hr_n'. apply Return_inv in Hr_n'. subst r_n'.
-  computes_to_econstructor. red; cbn. red in Hrel. subst r_o. reflexivity.
-Qed.
-
 
 Definition LessHistoryRelation (r_o r_n : sigT (@AllFinite PacketHistorySchema)) :=
   forall inp,
@@ -282,125 +144,77 @@ Lemma LessHistoryRelationRefl:
 Proof.
   unfold LessHistoryRelation; split; intros; assumption. Qed.
 
-Definition IncrMaxFreshIdx (r: sigT (@AllFinite PacketHistorySchema)) :=
-  S (fold_right (fun elem acc => max (elementIndex elem) acc) 0 (proj1_sig (projT2 ((projT2 r) Fin.F1)))).
-
-Lemma IncrMaxFreshIdx_Refine:
-  forall (r: sigT (@AllFinite PacketHistorySchema)),
-    refine
-      {idx: nat | UnConstrFreshIdx (GetUnConstrRelation (projT1 r) Fin.F1) idx}
-      (ret (IncrMaxFreshIdx r)).
-Proof.
-  intros r. pose (proj2_sig (projT2 ((projT2 r) Fin.F1))) as Hl.
-  destruct Hl as [Hmap [Heqv Hdup]].
-  intro idx; intro Hidx; computes_to_econstructor;
-    intro elem; intros Helem.
-  apply Return_inv in Hidx. apply Heqv in Helem.
-  unfold lt. rewrite <- Hidx. apply le_n_S.
-  apply fold_right_max_is_max; apply Helem.
-Qed.
-
 
 Theorem SharpenNoIncomingFilter:
   FullySharpened NoIncomingConnectionsFilter.
 Proof.
-  start sharpening ADT.
-  hone representation using (@DropQSConstraints_AbsR PacketHistorySchema).
-  - apply Constructor_DropQSConstraints.
-  - simplify with monad laws.
-    unfold Bind2.
-    simplify with monad laws.
-    Transparent QSInsert.
-    cbn.
+  start sharpening ADT. Transparent QSInsert.
+  drop_constraints_under_bind PacketHistorySchema ltac:(
+    intro v; intros Htemp;
+    match goal with
+      [H: DropQSConstraints_AbsR _ _ |- _] =>
+      apply (UnConstrPreservesFilterMethod _ _ _ _ H)
+    end;
+    apply Htemp).
 
-    etransitivity.
-    eapply refine_bind.
+  Definition myqidx:
+    Fin.t (numRawQSschemaSchemas PacketHistorySchema).
+    cbn. apply Fin.F1. Defined. Print myqidx.
+  hone_finite_under_bind PacketHistorySchema myqidx.
+
+  hone representation using LessHistoryRelation;
+    try simplify with monad laws.
+  - refine pick val
+           (existT _ (DropQSConstraints (QSEmptySpec _)) QSEmptyIsFinite).
+    subst H; reflexivity. apply LessHistoryRelationRefl.
+  - etransitivity. eapply refine_under_bind.
+    intros res Hres. cbn. eapply refine_bind.
+
+    Definition RefinedInsert
+               (r: sigT (@AllFinite PacketHistorySchema)) d :=
+      existT AllFinite (UpdateUnConstrRelation (projT1 r) Fin.F1
+                                               (EnsembleInsert
+                                                  {| elementIndex := IncrMaxFreshIdx r;
+                                                     indexedElement := icons2 d inil2 |}
+                                                  (GetUnConstrRelation (projT1 r) Fin.F1)))
+             (insert_finite_helper r Fin.F1
+                                   {| elementIndex := IncrMaxFreshIdx r;
+                                      indexedElement := icons2 d inil2 |}
+                                   (IncrMaxFreshIdx_Prop r)).
+
+    refine pick val
+           (if cf_cond OutgoingRule d
+            then (RefinedInsert r_n d)
+            else r_n).
     reflexivity.
-    unfold pointwise_relation.
-    intros.
 
-    etransitivity.
-    apply change_refine_form.
-    unfold QSInsert.
-    rewrite QSInsertSpec_UnConstr_refine; eauto; cycle 1;
-      try (refine pick val true; [reflexivity | cbv; intros; exact I]);
-      try (cbv -[refine]; intros; refine pick val true;
-        [simplify with monad laws; higher_order_reflexivity | eauto]).
-      * simplify with monad laws.
-        higher_order_reflexivity.
-      * etransitivity. eapply refine_bind. red; intros v Htemp.
-        apply (UnConstrPreservesFilterMethod r_o r_n d v H0). apply Htemp.
-        unfold pointwise_relation; intros. higher_order_reflexivity.
-        subst H. higher_order_reflexivity.
+    destruct (cf_cond OutgoingRule d) eqn:outrule.
+    red; intros inp Hinp. unfold RefinedInsert. split; intros.
 
-  - hone representation using (@FiniteTables_AbsR' PacketHistorySchema).
-    + simplify with monad laws.
-      refine pick val
-        (existT _ (DropQSConstraints (QSEmptySpec _)) QSEmptyIsFinite).
-      * subst H; higher_order_reflexivity.
-      * apply FiniteTables_AbsR'_QSEmptySpec.
-    + simplify with monad laws.
-      eapply refine_bind.
-      * red in H0; simpl in H0; rewrite H0.
-        higher_order_reflexivity.
-      * red; intros. red in H0. subst r_o.
-        eapply refine_under_bind_both.
-        apply IncrMaxFreshIdx_Refine.
-        intros idx Hidx; cbn.
-        rewrite FiniteTables_AbsR'_Insert; cbn; eauto.
-        simplify with monad laws. higher_order_reflexivity.
-        unfold FiniteTables_AbsR'. reflexivity.
+    cbn in H1. rewrite get_update_unconstr_eq in H1. red in H1. destruct H1. destruct H1.
+    { exists (@IncrMaxFreshIdx _ myqidx r_o). cbn. red. rewrite get_update_unconstr_eq. red. left. inversion H1. reflexivity. }
+    { cbn. rewrite get_update_unconstr_eq. red. unfold In. unfold EnsembleInsert. pose proof (H0 inp Hinp). unfold IndexedEnsemble_In in H2. unfold In in H2. assert (Hm: exists idx, GetUnConstrRelation (projT1 r_o) Fin.F1 {| elementIndex := idx; indexedElement := icons2 (value (ilist2_hd (icons2 (sINPUT :: inp)%Component inil2))) inil2 |}). { apply H2. exists x. apply H1. } destruct Hm. exists x0. right. apply H3. }
 
-    + hone representation using LessHistoryRelation;
-        try simplify with monad laws.
-      * refine pick val
-          (existT _ (DropQSConstraints (QSEmptySpec _)) QSEmptyIsFinite).
-        subst H; reflexivity. apply LessHistoryRelationRefl.
-      * etransitivity. eapply refine_under_bind.
-        intros res Hres. cbn. eapply refine_bind.
+    cbn in H1. rewrite get_update_unconstr_eq in H1. red in H1. destruct H1. destruct H1.
+    { exists (@IncrMaxFreshIdx _ myqidx r_n). cbn. red. rewrite get_update_unconstr_eq. red. left. inversion H1. reflexivity. }
+    { cbn. rewrite get_update_unconstr_eq. red. unfold In. unfold EnsembleInsert. pose proof (H0 inp Hinp). unfold IndexedEnsemble_In in H2. unfold In in H2. assert (Hm: exists idx, GetUnConstrRelation (projT1 r_n) Fin.F1 {| elementIndex := idx; indexedElement := icons2 (value (ilist2_hd (icons2 (sINPUT :: inp)%Component inil2))) inil2 |}). { apply H2. exists x. apply H1. } destruct Hm. exists x0. right. apply H3. }
 
-        Definition RefinedInsert
-                   (r: sigT (@AllFinite PacketHistorySchema)) d H :=
-          existT AllFinite (UpdateUnConstrRelation (projT1 r) Fin.F1
-            (EnsembleInsert
-               {| elementIndex := IncrMaxFreshIdx r;
-                  indexedElement := icons2 d inil2 |}
-               (GetUnConstrRelation (projT1 r) Fin.F1)))
-            (insert_finite_helper PacketHistorySchema r Fin.F1
-               {| elementIndex := IncrMaxFreshIdx r;
-                  indexedElement := icons2 d inil2 |} H).
+    red; intros inp Hinp. split; intros.
+
+    apply (H0 inp Hinp) in H1. cbn. rewrite get_update_unconstr_eq. red. red in H1. destruct H1. exists x. red. red. right. apply H1.
+
+    cbn in H1; rewrite get_update_unconstr_eq in H1. red in H1. destruct H1. red in H1. red in H1. destruct H1. inversion H1. rewrite <- H4 in outrule. rewrite outrule in Hinp. inversion Hinp. apply (H0 inp Hinp). red; exists x; red. apply H1.
+
+
+    red; intros. higher_order_reflexivity.
+    simplify with monad laws. eapply refine_bind.
+    apply (LessHistoryPreservesFilter d r_o r_n H0).
+    red; intros. higher_order_reflexivity.
+
+
+    
+  - hone representation using eq.
         
-        refine pick val
-               (if cf_cond OutgoingRule d
-                then (RefinedInsert r_n d _)
-                else r_n).
-        reflexivity.
-
-        destruct (cf_cond OutgoingRule d) eqn:outrule.
-        red; intros inp Hinp. unfold RefinedInsert. split; intros.
-
-        cbn in H1. rewrite get_update_unconstr_eq in H1. red in H1. destruct H1. destruct H1.
-        { exists (IncrMaxFreshIdx r_o). cbn. red. rewrite get_update_unconstr_eq. red. left. inversion H1. reflexivity. }
-        { cbn. rewrite get_update_unconstr_eq. red. unfold In. unfold EnsembleInsert. pose proof (H0 inp Hinp). unfold IndexedEnsemble_In in H2. unfold In in H2. assert (Hm: exists idx, GetUnConstrRelation (projT1 r_o) Fin.F1 {| elementIndex := idx; indexedElement := icons2 (value (ilist2_hd (icons2 (sINPUT :: inp)%Component inil2))) inil2 |}). { apply H2. exists x. apply H1. } destruct Hm. exists x0. right. apply H3. }
-
-        cbn in H1. rewrite get_update_unconstr_eq in H1. red in H1. destruct H1. destruct H1.
-        { exists (IncrMaxFreshIdx r_n). cbn. red. rewrite get_update_unconstr_eq. red. left. inversion H1. reflexivity. }
-        { cbn. rewrite get_update_unconstr_eq. red. unfold In. unfold EnsembleInsert. pose proof (H0 inp Hinp). unfold IndexedEnsemble_In in H2. unfold In in H2. assert (Hm: exists idx, GetUnConstrRelation (projT1 r_n) Fin.F1 {| elementIndex := idx; indexedElement := icons2 (value (ilist2_hd (icons2 (sINPUT :: inp)%Component inil2))) inil2 |}). { apply H2. exists x. apply H1. } destruct Hm. exists x0. right. apply H3. }
-
-        red; intros inp Hinp. split; intros.
-
-        apply (H0 inp Hinp) in H1. cbn. rewrite get_update_unconstr_eq. red. red in H1. destruct H1. exists x. red. red. right. apply H1.
-
-        cbn in H1; rewrite get_update_unconstr_eq in H1. red in H1. destruct H1. red in H1. red in H1. destruct H1. inversion H1. rewrite <- H4 in outrule. rewrite outrule in Hinp. inversion Hinp. apply (H0 inp Hinp). red; exists x; red. apply H1.
-
-
-        red; intros. higher_order_reflexivity.
-        simplify with monad laws. eapply refine_bind.
-        apply (LessHistoryPreservesFilter d r_o r_n H0).
-        red; intros. higher_order_reflexivity.
-
-
-      * 
         
 
 
